test/Tests.ml
@@ -32,11 +32,22 @@ let%expect_test "lazy_star_1" =
     0;
   [%expect {| Matched 6 characters ([0-6]) in 'aaaaab' (length=6) |}]
 
+let%expect_test "groups" =
+  test_regex
+    (   group (None, char 'a')
+    ||  group (None, char 'b'))
+    "ab"
+    0;
+  [%expect {|
+    Matched 1 characters ([0-1]) in 'ab' (length=2)
+    Group 1: 'a' ([0-1])
+    Group 2: undefined |}]
+
 
 let%expect_test "capture_reset" =
   test_regex
-    !*(   group (1, char 'a')
-    ||  group (2, char 'b'))
+    !*( group (None, char 'a')
+    ||  group (None, char 'b'))
     "ab"
     0;
   [%expect {|
@@ -135,80 +146,80 @@ let%expect_test "neglookbehind_0_neg" =
 
 let%expect_test "backref_0_pos" =
   test_regex
-    (group (0, (char 'a')) -- !$ 0)
+    (group (None, (char 'a')) -- !$ 1)
     "aa"
     0;
   [%expect {|
     Matched 2 characters ([0-2]) in 'aa' (length=2)
-    Group 0: 'a' ([0-1]) |}]
+    Group 1: 'a' ([0-1]) |}]
 
 let%expect_test "backref_0_neg_0" =
   test_regex
-    (group (0, (char 'a')) -- !$ 0)
+    (group (None, (char 'a')) -- !$ 1)
     "ab"
     0;
   [%expect {| No match on 'ab' |}]
 
 let%expect_test "backref_0_neg_1" =
   test_regex
-    (group (0, (char 'a')) -- !$ 0)
+    (group (None, (char 'a')) -- !$ 1)
     "a"
     0;
   [%expect {| No match on 'a' |}]
 
 let%expect_test "backref_undefined" =
   test_regex
-    ((group (0, (char 'a')) || group (1, (char 'b'))) -- !$ 1)
+    ((group (None, (char 'a')) || group (None, (char 'b'))) -- !$ 2)
     "aa"
     0;
   [%expect {|
     Matched 1 characters ([0-1]) in 'aa' (length=2)
-    Group 0: 'a' ([0-1])
-    Group 1: undefined |}]
+    Group 1: 'a' ([0-1])
+    Group 2: undefined |}]
 
 let%expect_test "backref_multiple" =
   test_regex
-    (group (0, (char 'a')) -- !$ 0 -- !$ 1 -- group (1, (char 'b')) -- !$ 0 -- !$ 1)
+    (group (None, (char 'a')) -- !$ 1 -- !$ 2 -- group (None, (char 'b')) -- !$ 1 -- !$ 2)
     "aabab"
     0;
   [%expect {|
     Matched 5 characters ([0-5]) in 'aabab' (length=5)
-    Group 0: 'a' ([0-1])
-    Group 1: 'b' ([2-3]) |}]
+    Group 1: 'a' ([0-1])
+    Group 2: 'b' ([2-3]) |}]
 
 let%expect_test "backref_long_pos" =
   test_regex
-    (group (0, (char 'a') -- (char 'b') -- (char 'a')) -- !$ 0)
+    (group (None, (char 'a') -- (char 'b') -- (char 'a')) -- !$ 1)
     "abaaba"
     0;
   [%expect {|
     Matched 6 characters ([0-6]) in 'abaaba' (length=6)
-    Group 0: 'aba' ([0-3]) |}]
+    Group 1: 'aba' ([0-3]) |}]
 
 let%expect_test "backref_long_neg_0" =
   test_regex
-    (group (0, (char 'a') -- (char 'b') -- (char 'a')) -- !$ 0)
+    (group (None, (char 'a') -- (char 'b') -- (char 'a')) -- !$ 1)
     "abaab"
     0;
   [%expect {| No match on 'abaab' |}]
 
 let%expect_test "backref_long_neg_1" =
 test_regex
-  (group (0, (char 'a') -- (char 'b') -- (char 'a')) -- !$ 0)
+  (group (None, (char 'a') -- (char 'b') -- (char 'a')) -- !$ 1)
   "abacba"
   0;
 [%expect {| No match on 'abacba' |}]
 
 let%expect_test "backref_long_neg_2" =
   test_regex
-    (group (0, (char 'a') -- (char 'b') -- (char 'a')) -- !$ 0)
+    (group (None, (char 'a') -- (char 'b') -- (char 'a')) -- !$ 1)
     "abaaca"
     0;
   [%expect {| No match on 'abaaca' |}]
 
 let%expect_test "backref_long_neg_3" =
   test_regex
-    (group (0, (char 'a') -- (char 'b') -- (char 'a')) -- !$ 0)
+    (group (None, (char 'a') -- (char 'b') -- (char 'a')) -- !$ 1)
     "abaabc"
     0;
   [%expect {| No match on 'abaabc' |}]
