MECMAR/spec/Patterns.v
@@ -1,3 +1,4 @@
+From Coq Require Import List Program.Equality.
 From Warblre Require Import Base Notation.
 
 (** 22.2.1 Patterns *)
@@ -56,6 +57,118 @@ Module Patterns.
   | Disjunction (r1 r2: Regex)
   | Quantified (r: Regex) (q: Quantifier)
   | Seq (r1 r2: Regex)
+  | Group (name: option GroupName) (r: Regex)
+  (* Assertions: ^ $ \b \B *)
+  | Lookahead (r: Regex)
+  | NegativeLookahead (r: Regex)
+  | Lookbehind (r: Regex)
+  | NegativeLookbehind (r: Regex)
+  | BackReference (id: positive_integer).
+
+  Inductive RegexContextLayer :=
+  | Disjunction_left (r: Regex)
+  | Disjunction_right (l: Regex)
+  | Quantified_inner (q: Quantifier)
+  | Seq_left (r: Regex)
+  | Seq_right (l: Regex)
+  | Group_inner (name: option GroupName)
+  | Lookahead_inner
+  | NegativeLookahead_inner
+  | Lookbehind_inner
+  | NegativeLookbehind_inner.
+
+  Notation RegexContext := (list RegexContextLayer).
+  (* Definition Node: Type := RegexTree * RegexContext. *)
+
+  Fixpoint zip (focus: Regex) (ctx: RegexContext): Regex :=
+    match ctx with
+    | nil => focus
+    | h :: t =>
+      zip (match h with
+      | Disjunction_left r => Disjunction focus r
+      | Disjunction_right l => Disjunction l focus
+      | Quantified_inner q => Quantified focus q
+      | Seq_left r => Seq focus r
+      | Seq_right l => Seq l focus
+      | Group_inner name => Group name focus
+      | Lookahead_inner => Lookahead focus
+      | NegativeLookahead_inner => NegativeLookahead focus
+      | Lookbehind_inner => Lookbehind focus
+      | NegativeLookbehind_inner => NegativeLookbehind focus
+      end) t
+    end.
+
+  Definition Root (r f: Regex) (ctx: RegexContext) := r = zip f ctx.
+
+  Module Root.
+    Lemma id: forall r, Root r r nil.
+    Proof. intros. reflexivity. Qed.
+  End Root.
+
+  Module Zip.
+    Lemma concat: forall ctx0 ctx1 r, (zip (zip r ctx0) ctx1) = zip r (ctx0 ++ ctx1).
+    Proof.
+      induction ctx0; intros ctx1 r.
+      - reflexivity.
+      - cbn. rewrite IHctx0. reflexivity.
+    Qed.
+
+    Lemma focus_injection: forall ctx r0 r1, zip r0 ctx = zip r1 ctx -> r0 = r1.
+    Proof.
+      induction ctx; intros r0 r1 Ineq.
+      - assumption.
+      - cbn in Ineq.
+        specialize IHctx with (1 := Ineq); destruct a; injection IHctx as ->; reflexivity.
+    Qed.
+
+    Lemma focus_bijection: forall ctx r0 r1, zip r0 ctx = zip r1 ctx <-> r0 = r1.
+    Proof. intros. split; intros. - eapply focus_injection. eassumption. - subst. reflexivity. Qed.
+
+    Module Down.
+      Lemma disjunction_left: forall root r f ctx, Root root (Disjunction f r) ctx -> Root root f (Disjunction_left r :: ctx).
+      Proof. intros. cbn. assumption. Qed.
+      Lemma disjunction_right: forall root l f ctx, Root root (Disjunction l f) ctx -> Root root f (Disjunction_right l :: ctx).
+      Proof. intros. cbn. assumption. Qed.
+
+      Lemma seq_left: forall root r f ctx, Root root (Seq f r) ctx -> Root root f (Seq_left r :: ctx).
+      Proof. intros. cbn. assumption. Qed.
+      Lemma seq_right: forall root l f ctx, Root root (Seq l f) ctx -> Root root f (Seq_right l :: ctx).
+      Proof. intros. cbn. assumption. Qed.
+
+      Lemma quantified_inner: forall root q f ctx, Root root (Quantified f q) ctx -> Root root f (Quantified_inner q :: ctx).
+      Proof. intros. cbn. assumption. Qed.
+      Lemma group_inner: forall root id f ctx, Root root (Group id f) ctx -> Root root f (Group_inner id :: ctx).
+      Proof. intros. cbn. assumption. Qed.
+
+      Lemma lookahead_inner: forall root f ctx, Root root (Lookahead f) ctx -> Root root f (Lookahead_inner :: ctx).
+      Proof. intros. cbn. assumption. Qed.
+      Lemma negativeLookahead_inner: forall root f ctx, Root root (NegativeLookahead f) ctx -> Root root f (NegativeLookahead_inner :: ctx).
+      Proof. intros. cbn. assumption. Qed.
+      Lemma lookbehind_inner: forall root f ctx, Root root (Lookbehind f) ctx -> Root root f (Lookbehind_inner :: ctx).
+      Proof. intros. cbn. assumption. Qed.
+      Lemma negativeLookbehind_inner: forall root f ctx, Root root (NegativeLookbehind f) ctx -> Root root f (NegativeLookbehind_inner :: ctx).
+      Proof. intros. cbn. assumption. Qed.
+    End Down.
+
+    Create HintDb down.
+    #[export]
+    Hint Resolve Down.disjunction_left Down.disjunction_right: down.
+    #[export]
+    Hint Resolve Down.seq_left Down.seq_right: down.
+    #[export]
+    Hint Resolve Down.quantified_inner Down.group_inner: down.
+    #[export]
+    Hint Resolve Down.lookahead_inner Down.negativeLookahead_inner Down.lookbehind_inner Down.negativeLookbehind_inner: down.
+
+    Ltac down := auto with down.
+  End Zip.
+
+(*   Inductive ZippedRegexPattern :=
+  | Empty
+  | Char (chr: Character)
+  | Disjunction (r1 r2: Regex)
+  | Quantified (r: Regex) (q: Quantifier)
+  | Seq (r1 r2: Regex)
   | Group (id: nat) (r: Regex)
   (* Assertions: ^ $ \b \B *)
   | Lookahead (r: Regex)
@@ -64,9 +177,21 @@ Module Patterns.
   | NegativeLookbehind (r: Regex)
   | BackReference (id: nat).
 
-(*   Module Regex.
-    Definition eqb (l r: Regex): {l = r} + {~ l = r}.
-    Proof. decide equality; (apply CharacterClass.eqb + apply Quantifier.eqb + (repeat decide equality)). Defined.
-  End Regex. *)
+  Definition down (r: Regex): ZippedRegexPattern :=
+    let (r, ctx) := r in
+    match r with
+    | Empty_p => Empty
+    | Char_p chr => Char chr
+    | Disjunction_p l r => Disjunction (l, Disjunction_left r :: ctx) (r, Disjunction_right l :: ctx)
+    | Quantified_p r q => Quantified (r, Quantified_inner q :: ctx) q
+    | Seq_p l r => Seq (l, Seq_left r :: ctx) (r, Seq_right l :: ctx)
+    | Group_p id r => Group id (r, Group_inner id :: ctx)
+    | Lookahead_p r => Lookahead (r, Lookahead_inner :: ctx)
+    | NegativeLookahead_p r => Lookahead (r, Lookahead_inner :: ctx)
+    | Lookbehind_p r  => Lookbehind (r, Lookbehind_inner :: ctx)
+    | NegativeLookbehind_p r  => NegativeLookbehind (r, NegativeLookbehind_inner :: ctx)
+    | BackReference_p id  => BackReference id
+    end. *)
+
 End Patterns.
 Export Patterns.
