MECMAR/spec/StaticSemantics.v
@@ -23,19 +23,40 @@ Module StaticSemantics.
   | SyntaxError.
 
   (** 22.2.1.2 Static Semantics: CountLeftCapturingParensWithin *)
-  Definition countLeftCapturingParensWithin (r: Regex): non_neg_integer := (*countLeftCapturingParensWithin_rec 0 r.*)
-    List.fold_left (fun acc r => match r with
-      | Group _ _ => acc + 1
-      | _ => acc
-      end) (pre_order_walk r) 0.
-
-  Definition capturingGroupsWithin (r: Regex): list nat :=
-    List.flat_map (fun r => match r with
-      | Group id _ => id :: nil
-      | _ => nil
-      end) (pre_order_walk r).
+  Fixpoint countLeftCapturingParensWithin_impl (r: Regex): non_neg_integer :=
+    match r with
+    | Empty => 0
+    | Char _ => 0
+    | Disjunction r1 r2 => (countLeftCapturingParensWithin_impl r1) + (countLeftCapturingParensWithin_impl r2)
+    | Quantified r0 _ => countLeftCapturingParensWithin_impl r0
+    | Seq r1 r2 => (countLeftCapturingParensWithin_impl r1) + (countLeftCapturingParensWithin_impl r2)
+    | Group _ r0 => 1 + (countLeftCapturingParensWithin_impl r0)
+    | Lookahead r0 => countLeftCapturingParensWithin_impl r0
+    | NegativeLookahead r0 => countLeftCapturingParensWithin_impl r0
+    | Lookbehind r0 => countLeftCapturingParensWithin_impl r0
+    | NegativeLookbehind r0 => countLeftCapturingParensWithin_impl r0
+    | BackReference _ => 0
+    end.
+  Definition countLeftCapturingParensWithin (r: Regex) (ctx: RegexContext): non_neg_integer := countLeftCapturingParensWithin_impl r.
 
   (** 22.2.1.3 Static Semantics: CountLeftCapturingParensBefore *)
+  Fixpoint countLeftCapturingParensBefore_impl (ctx: RegexContext): non_neg_integer :=
+    match ctx with
+    | nil => 0
+    | h :: t => (countLeftCapturingParensBefore_impl t) + match h with
+      | Disjunction_left _ => 0
+      | Disjunction_right l => countLeftCapturingParensWithin_impl l
+      | Quantified_inner _ => 0
+      | Seq_left _ => 0
+      | Seq_right l => countLeftCapturingParensWithin_impl l
+      | Group_inner _ => 0
+      | Lookahead_inner => 0
+      | NegativeLookahead_inner => 0
+      | Lookbehind_inner => 0
+      | NegativeLookbehind_inner => 0
+      end
+    end.
+  Definition countLeftCapturingParensBefore (r: Regex) (ctx: RegexContext): non_neg_integer := countLeftCapturingParensBefore_impl ctx.
 (*   Fixpoint countLeftCapturingParensBefore_rec (target: Regex) (acc: non_neg_integer) (walk: list Regex): option non_neg_integer :=
     match walk with
     | nil => None
