MECMAR/utils/List.v
@@ -183,11 +183,11 @@ Module List.
         - assert (Pos.to_nat (p + 1) = S (Pos.to_nat p)) as -> by lia. apply Nat.cons.
         - lia.
       Qed.
-      
+
       Lemma repeat {T F: Type} {failure: Result.AssertionError F}: forall n v i v',
         indexing (@List.repeat T v n) i = Success v' -> v = v'.
       Proof. intros n v i v' H. destruct i. - apply Nat.repeat with (1 := H). - apply Nat.repeat with (1 := H). - apply Indexing.Int.success_bounds in H. lia. Qed.
-      
+
       (** Int only theorems *)
 
       Lemma of_nat {T F: Type} {failure: Result.AssertionError F}: forall (ls: list T) (i: nat), indexing ls (Z.of_nat i) = Nat.indexing ls i.
@@ -403,291 +403,6 @@ Module List.
 
       End Batch.
     End Nat.
-(* 
-    Definition updating {T F: Type} (ls: list T) (i: Z) (v: T) {failure: Result.AssertionError F}: Result.Result (list T) F := match i with
-    | Z0 => updating_nat ls 0 v
-    | Zpos i => updating_nat ls (Pos.to_nat i) v
-    | Zneg _ => Result.assertion_failed
-    end.
-
-    Definition batch_updating0_nat {T F: Type} {_: Result.AssertionError F} (ls: Result (list T) F) (is: list nat) (v: T) := List.FoldResult.fold_left_result0 (fun ls i => List.Updating.updating_nat ls i v) is ls.
-    Definition batch_updating_nat {T F: Type} {_: Result.AssertionError F} (ls: list T) (is: list nat) (v: T) := List.FoldResult.fold_left_result (fun ls i => List.Updating.updating_nat ls i v) is ls.
-
-    Definition batch_updating0 {T F: Type} {_: Result.AssertionError F} (ls: Result (list T) F) (is: list Z) (v: T) := List.FoldResult.fold_left_result0 (fun ls i => List.Updating.updating ls i v) is ls.
-    Definition batch_updating {T F: Type} {_: Result.AssertionError F} (ls: list T) (is: list Z) (v: T) := List.FoldResult.fold_left_result (fun ls i => List.Updating.updating ls i v) is ls.
-
-    Lemma batch_nat_cons {T F: Type} {_: Result.AssertionError F}: forall (ls: list T) (i: nat) (is: list nat) (v: T),
-      batch_updating_nat ls (i :: is) v = let! ls' =<< updating_nat ls i v in batch_updating_nat ls' is v.
-    Proof. intros ls i is v. unfold batch_updating_nat. rewrite -> FoldResult.cons. reflexivity. Qed.
-    Lemma batch_cons {T F: Type} {_: Result.AssertionError F}: forall (ls: list T) (i: Z) (is: list Z) (v: T),
-      batch_updating ls (i :: is) v = let! ls' =<< updating ls i v in batch_updating ls' is v.
-    Proof. intros ls i is v. unfold batch_updating. rewrite -> FoldResult.cons. reflexivity. Qed.
-
-    Lemma success_length_nat {T F: Type} {f: Result.AssertionError F}: forall (ls ls': list T) (i: nat) (v: T), updating_nat ls i v = Success ls' -> (length ls) = (length ls').
-    Proof.
-      intros ls. induction ls; intros ls' i v H.
-      - Result.assertion_failed_helper.
-      - destruct i.
-        + injection H as <-. reflexivity.
-        + cbn in *. destruct (updating_nat ls i v) eqn:Eq_updated; try discriminate.
-          injection H as <-. cbn. f_equal.
-          apply IHls with (1 := Eq_updated).
-    Qed.
-
-    Lemma success_length {T F: Type} {f: Result.AssertionError F}: forall (ls ls': list T) (i: Z) (v: T), updating ls i v = Success ls' -> (length ls) = (length ls').
-    Proof. intros ls ls' i v H. induction i using pseudo_nat_ind. - apply success_length_nat with (1 := H). - apply success_length_nat with (1 := H). - Result.assertion_failed_helper. Qed.
-
-    Lemma of_nat {T F: Type} {f: Result.AssertionError F}: forall (ls: list T) (i: nat) (v: T), updating_nat ls i v = updating ls (Z.of_nat i) v.
-    Proof. intros. destruct i; cbn; try rewrite -> SuccNat2Pos.id_succ; reflexivity. Qed.
-
-    Lemma failure_bounds_nat: forall {T F: Type} {failure: Result.AssertionError F} (ls: list T) (i: nat) (v: T), @updating_nat T F ls i v failure = Result.assertion_failed <-> (length ls <= i )%nat.
-    Proof. 
-      intros T F failure.
-      induction ls; intros.
-      - split; cbn; [ lia | easy ].
-      - split; cbn.
-        + focus § _ [] _ -> _ § auto destruct; Result.assertion_failed_helper.
-          intros [=->]. rewrite -> IHls in AutoDest_0. lia.
-        + intros. focus § _ [] _ § auto destruct.
-          * lia.
-          * destruct (IHls n v) as [ _ IHls' ].
-            rewrite -> IHls' in AutoDest_0 by lia.
-            Result.assertion_failed_helper.
-          * rewrite <- AutoDest_0. rewrite -> IHls. lia.
-    Qed.
-
-    Lemma failure_is_assertion_nat: forall {T F: Type} {failure: Result.AssertionError F} (ls: list T) (i: nat) (f: F) (v: T),
-      updating_nat ls i v = Result.Failure f -> {| Result.f := f |} = failure.
-    Proof.
-      induction ls; intros i f v; destruct i; cbn in *; Result.assertion_failed_helper; first[ intros [=->] | intros H ]; try easy.
-      destruct (updating_nat ls i v) eqn:Eq.
-      - discriminate.
-      - clean_injection H. specialize IHls with (1 := Eq). subst. Result.assertion_failed_helper.
-    Qed.
-
-    Lemma failure_kind_nat: forall {T F: Type} {failure: Result.AssertionError F} (ls: list T) (i: nat) (f: F) (v: T),
-      updating_nat ls i v = Result.Failure f -> updating_nat ls i v = Result.assertion_failed.
-    Proof. intros. pose proof (failure_is_assertion_nat ls i f v H). Result.assertion_failed_helper. Qed.
-
-(*     Lemma failure_kind {T F: Type} {failure: Result.AssertionError F}: forall (ls: list T) (i: Z) (f: F) (v: T),
-      updating ls i v = Result.Failure f -> updating ls i v = Result.assertion_failed.
-    Proof. intros ls i f v H. destruct i. - apply failure_kind_nat with (f := f). apply H. - apply failure_kind_nat with (f := f). apply H. - Result.assertion_failed_helper. Qed.
- *)
-    Lemma failure_bounds: forall {T F: Type} {failure: Result.AssertionError F} (ls: list T) (i: Z) (v: T), @updating T F ls i v failure = Result.assertion_failed <-> (i < 0 \/ Z.of_nat (length ls) <= i )%Z.
-    Proof.
-      intros. split.
-      - intros. destruct i; cbn in H.
-        + apply failure_bounds_nat in H. right. lia.
-        + apply failure_bounds_nat in H. right. lia.
-        + left. lia.
-      - intros [ i_leq_0 | len_le_i ]; destruct i; cbn.
-        + lia.
-        + lia.
-        + reflexivity.
-        + destruct ls; cbn in *; try lia. reflexivity.
-        + apply failure_bounds_nat. lia.
-        + lia.
-    Qed.
-
-    Lemma batch_failure_bounds {T F: Type} {f: Result.AssertionError F}: forall (is: list Z) (ls: list T) (v: T),
-      @batch_updating T F f ls is v = Result.assertion_failed
-      ->
-      (exists j i, Indexing.indexing is j = Success i /\ (i < 0 \/ Z.of_nat (length ls) <= i) )%Z.
-    Proof.
-      assert (forall (is: list Z) (ls: list T) (v: T),
-        @batch_updating T F f ls is v = Result.assertion_failed
-        ->
-        (exists j i, Indexing.indexing is j = Success i /\ (i < 0 \/ Z.of_nat (length ls) <= i) )%Z
-      ) as LtR. {
-        induction is; intros ls v Eq_failure.
-        - Result.assertion_failed_helper.
-        - rewrite batch_cons in Eq_failure.
-          destruct (updating ls a v) eqn:Eq_updated.
-          + apply IHis in Eq_failure. destruct Eq_failure as [ j [ i [ Eq_indexed Ineq_i ]]].
-            pose proof (Indexing.success_bounds _ _ _ Eq_indexed) as B_j.
-            exists (j + 1). exists i.
-            split. * rewrite -> Indexing.cons0; [ apply Eq_indexed | lia ]. * apply Updating.success_length in Eq_updated. lia.
-          + exists 0. exists a. split. * reflexivity. * rewrite <- failure_bounds with (v := v). Result.assertion_failed_helper.
-      }
-      apply LtR.
-    Qed.
-    
-    Lemma batch_nat_failure_bounds {T F: Type} {f: Result.AssertionError F}: forall (is: list nat) (ls: list T) (v: T),
-      @batch_updating_nat T F f ls is v = Result.assertion_failed
-      ->
-      (exists j i, Indexing.indexing is j = Success i /\ (length ls <= i))%nat.
-    Proof.
-      assert (forall (is: list nat) (ls: list T) (v: T),
-        @batch_updating_nat T F f ls is v = Result.assertion_failed
-        ->
-        (exists j i, Indexing.indexing is j = Success i /\ (length ls <= i) )%nat
-      ) as LtR. {
-        induction is; intros ls v Eq_failure.
-        - Result.assertion_failed_helper.
-        - rewrite batch_nat_cons in Eq_failure.
-          destruct (updating_nat ls a v) eqn:Eq_updated.
-          + apply IHis in Eq_failure. destruct Eq_failure as [ j [ i [ Eq_indexed Ineq_i ]]].
-            pose proof (Indexing.success_bounds _ _ _ Eq_indexed) as B_j.
-            exists (j + 1). exists i.
-            split. * rewrite -> Indexing.cons0; [ apply Eq_indexed | lia ]. * apply Updating.success_length_nat in Eq_updated. lia.
-          + exists 0. exists a. split. * reflexivity. * rewrite <- failure_bounds_nat with (v := v). Result.assertion_failed_helper.
-      }
-      apply LtR.
-    Qed.
-
-    Lemma failure_is_assertion: forall {T F: Type} {failure: Result.AssertionError F} (ls: list T) (i: Z) (f: F) (v: T),
-      updating ls i v = Result.Failure f -> {| Result.f := f |} = failure.
-    Proof.
-      intros. destruct i.
-      - apply failure_is_assertion_nat in H. assumption.
-      - apply failure_is_assertion_nat in H. assumption.
-      - cbn in H. Result.assertion_failed_helper.
-    Qed.
-
-    Lemma failure_kind: forall {T F: Type} {failure: Result.AssertionError F} (ls: list T) (i: Z) (f: F) (v: T),
-      updating ls i v = Result.Failure f -> updating ls i v = Result.assertion_failed.
-    Proof. intros. pose proof (failure_is_assertion ls i f v H). Result.assertion_failed_helper. Qed.
-
-    Lemma batch_failure_kind: forall {T F: Type} {failure: Result.AssertionError F} (is: list Z) (ls: list T) (f: F) (v: T),
-      batch_updating ls is v = Result.Failure f -> batch_updating ls is v = Result.assertion_failed.
-    Proof.
-      induction is; intros ls f v H.
-      - Result.assertion_failed_helper.
-      - rewrite -> batch_cons.
-        destruct (updating ls a v) eqn:Eq_updated.
-        * rewrite -> Updating.batch_cons in H. rewrite -> Eq_updated in H. apply IHis with (1 := H).
-        * pose proof (failure_kind _ _ _ _ Eq_updated) as Tmp. Result.assertion_failed_helper. rewrite -> Eq_updated in Tmp. injection Tmp as ->.
-          reflexivity.
-    Qed.
-
-    Lemma success_bounds: forall {T F: Type} {failure: Result.AssertionError F} (ls: list T) (i: Z) (v: T),
-      (exists ls', updating ls i v = Success ls') <-> (0 <= i /\ i < (Z.of_nat (length ls)) )%Z.
-    Proof. intros T F f. split.
-      - intros [ ls' H ]. pose proof (failure_bounds ls i) as [ _ Falsum ].
-        destruct ( (0 <=? i) && (i <? Z.of_nat (length ls)))%Z eqn:Bounds.
-        + Zhelper. lia.
-        + hypotheses_reflector.
-          * rewrite -> Z.leb_gt in H0. specialize (Falsum (or_introl H0)). destruct f. rewrite -> H in *. discriminate.
-          * rewrite -> Z.ltb_ge in H0. specialize (Falsum (or_intror H0)). destruct f. rewrite -> H in *. discriminate.
-      - intros [ Leq_0_i Le_i_len ]. pose proof (failure_bounds ls i v) as [ Falsum _ ].
-        destruct i eqn:Eq_i.
-        + destruct ls eqn:Eq_ls; cbn in *; try lia. exists (v :: l). reflexivity.
-        + destruct (updating ls (Z.pos p) v) eqn:Eq_indexed in |- *.
-          * exists s. reflexivity.
-          * apply failure_kind in Eq_indexed. specialize (Falsum Eq_indexed).
-            destruct Falsum; lia.
-        + lia.
-    Qed.
-
-    Lemma nil {T F: Type} {failure: Result.AssertionError F}: forall (i: Z) (v: T), updating nil i v = Result.assertion_failed.
-    Proof. intros. destruct i; reflexivity. Qed.
-
-    Lemma cons_nat {T F: Type} {failure: Result.AssertionError F}: forall (t: list T) (h: T) (i: nat) (v: T),
-      updating_nat (h :: t) (S i) v = (let! t' =<< updating_nat t i v in Success (h :: t')).
-    Proof.
-      induction t; intros h i v.
-      - reflexivity.
-      - destruct i eqn:Eq_i.
-        + reflexivity.
-        + rewrite -> IHt. reflexivity.
-    Qed.
-
-    Lemma cons {T F: Type} {failure: Result.AssertionError F}: forall (h: T) (t: list T) (i: Z) (v: T),
-      0 <= i -> updating (h :: t) (i + 1) v = (let! t' =<< updating t i v in Success (h :: t')).
-    Proof.
-      intros h t i v Ineq_i.
-      destruct i eqn:Eq_i; cbn -[updating_nat].
-      - assert (Pos.to_nat 1 = 1%nat) as -> by lia.
-        rewrite -> cons_nat. reflexivity.
-      - assert (Pos.to_nat (p + 1) = S (Pos.to_nat p)) as -> by lia.
-        rewrite -> cons_nat. reflexivity.
-      - lia.
-    Qed.
-
-    Lemma cons_of_nat {T F: Type} {failure: Result.AssertionError F}: forall (h: T) (t: list T) (i: nat) (v: T),
-      updating (h :: t) (Z.of_nat (S i)) v = (let! t' =<< updating t (Z.of_nat i) v in Success (h :: t')).
-    Proof. intros h t i v. assert (Z.of_nat (S i) = Z.of_nat i + 1) as -> by lia. apply cons. lia. Qed.
-
-    Lemma indexing_updated_same {T F: Type} {failure: Result.AssertionError F}: forall i (ls: list T) v ls',
-      updating ls i v = Success ls' -> Indexing.indexing ls' i = Success v.
-    Proof.
-      induction i using pseudo_nat_ind; intros ls v ls' H; (destruct ls; [ Result.assertion_failed_helper | ]).
-      - injection H as [=<-]. reflexivity.
-      - cbn in H. rewrite -> SuccNat2Pos.id_succ in H.
-        focus § _ [] _ § auto destruct in H.
-        injection H as [=<-].
-        rewrite -> Indexing.cons_of_nat_succ.
-        apply IHi with (ls := ls).
-        rewrite <- Updating.of_nat. assumption.
-      - Result.assertion_failed_helper.
-    Qed.
-
-    Lemma indexing_updated_other {T F: Type} {failure: Result.AssertionError F}: forall i (ls: list T) v ls',
-      updating ls i v = Success ls' -> forall j, i <> j -> Indexing.indexing ls' j = Indexing.indexing ls j.
-    Proof.
-      induction i using pseudo_nat_ind; intros ls v ls' H j Ineq_j; (destruct ls; [ solve[ Result.assertion_failed_helper ] | ]).
-      - injection H as [=<-]. induction j using pseudo_nat_ind.
-        + lia.
-        + focus § _ _ [] § do (fun t => destruct t eqn:Eq_indexed).
-          * rewrite -> Indexing.cons_of_nat_succ in *. assumption.
-          * replace (Z.of_nat (S n)) with ((Z.of_nat n) + 1) in * by lia.
-            rewrite -> Indexing.cons0 in * by lia.
-            assumption.
-        + cbn. reflexivity.
-      - rewrite -> cons_of_nat in H. focus § _ [] _ § auto destruct in H.
-        injection H as <-.
-        destruct j; try reflexivity.
-        assert (Z.pos p = (Z.pos p - 1) + 1) as -> by lia.
-        do 2 rewrite -> Indexing.cons0 by lia.
-        apply IHi with (v := v).
-        + assumption.
-        + lia.
-      - Result.assertion_failed_helper.
-    Qed.
-
-    Lemma prop_preservation {T F: Type} {failure: Result.AssertionError F}: forall (ls: list T) i v ls' P,
-      Forall ls P ->
-      P v ->
-      updating ls i v = Success ls' ->
-      Forall ls' P.
-    Proof.
-      intros ls i v ls' P H Pv Eq_ls' j w Eq_indexed.
-      destruct (Z.eq_dec i j) as [ Eq_ij | Neq_ij ].
-      - subst. apply indexing_updated_same in Eq_ls'.
-        rewrite Eq_ls' in *. injection Eq_indexed as ->.
-        assumption.
-      - apply H with (i := j).
-        rewrite <- Eq_indexed. symmetry.
-        apply indexing_updated_other with (1 := Eq_ls') (2 := Neq_ij).
-    Qed.
-    
-
-    Lemma batch_equiv {T F: Type} {_: Result.AssertionError F}: forall ls is v,
-      @batch_updating0 T F _ (Success ls) is v = @batch_updating T F _ ls is v.
-    Proof. reflexivity. Qed.
-
-    Lemma batch_prop_preservation {T F: Type} {failure: Result.AssertionError F}: forall is (ls: list T) v ls' P,
-      Forall ls P ->
-      P v ->
-      batch_updating ls is v = Success ls' ->
-      Forall ls' P.
-    Proof.
-      induction is; intros ls v ls' P FP_ls P_v Eq_ls'.
-      - cbn in Eq_ls'. injection Eq_ls' as <-. assumption.
-      - cbn in Eq_ls'.
-        focus § _ [] _ § replace with (batch_updating0 (updating ls a v) is v) in Eq_ls'.
-        destruct (updating ls a v) eqn:Eq_updated.
-        + apply IHis with (2 := P_v) (3 := Eq_ls').
-          intros i w Eq_indexed.
-          destruct (Z.eq_dec a i) as [ Eq_ai | Neq_ai ].
-          * subst. pose proof (indexing_updated_same _ _ _ _ Eq_updated).
-            assert (v = w) as -> by congruence. assumption.
-          * pose proof (indexing_updated_other _ _ _ _ Eq_updated _ Neq_ai).
-            apply (FP_ls i w). congruence.
-        + pose proof (FoldResult.zero_failure0 (fun ls i => updating ls i v) is f).
-          unfold batch_updating0 in Eq_ls'. congruence.
-    Qed.
-  End Updating. *)
   End Update.
 
   Module Exists.
@@ -712,59 +427,110 @@ Module List.
   End Exists.
 
   Module Range.
-    Module Impl.
-      Fixpoint range (base: Z) (l: nat) := match l with
-      | 0%nat => nil
-      | S l' => base :: (range (base + 1) l')
-      end.
+    Module Nat.
+      Definition IsRange (from to: nat) (ls: list nat) :=
+        (forall (F: Type) (f: Result.AssertionError F) z, (from <= z < to)%nat -> Indexing.Nat.indexing ls (z - from)%nat = Success z).
 
-      Lemma length: forall l b, length (range b l) = l.
-      Proof. induction l; intros b; cbn. - reflexivity. - rewrite -> IHl. reflexivity. Qed.
+      Module Length.
+        Fixpoint range (base: nat) (l: nat) := match l with
+        | 0%nat => nil
+        | S l' => base :: (range (base + 1) l')
+        end.
 
-      Lemma indexing {F: Type} {f: Result.AssertionError F}: forall i b l v,
-        Indexing.Int.indexing (range b l) i = Success v -> v = (b + i).
-      Proof.
-        induction i using pseudo_nat_ind.
-        - intros. cbn in *.
-          destruct l; try Result.assertion_failed_helper. cbn in *.
-          injection H as [=->]. lia.
-        - intros. cbn in *. rewrite -> SuccNat2Pos.id_succ in H.
-          destruct l; try Result.assertion_failed_helper. cbn in *.
-          specialize (IHi (b + 1) l). cbn in IHi.
-          rewrite -> Indexing.Int.of_nat in *. specialize (IHi _ H).
-          lia.
-        - intros. cbn in H. Result.assertion_failed_helper.
-      Qed.
-    End Impl.
+        Lemma length: forall l b, length (range b l) = l.
+        Proof. induction l; intros b; cbn. - reflexivity. - rewrite -> IHl. reflexivity. Qed.
 
-    Definition IsRange (from to: Z) (ls: list Z) :=
-      (forall (F: Type) (f: Result.AssertionError F) z, from <= z < to -> Indexing.Int.indexing ls (z - from) = Success z).
+        Lemma indexing {F: Type} {f: Result.AssertionError F}: forall i b l v,
+          Indexing.Nat.indexing (range b l) i = Success v -> v = (b + i)%nat.
+        Proof.
+          induction i.
+          - intros. cbn in *.
+            destruct l; try Result.assertion_failed_helper. cbn in *.
+            injection H as [=->]. lia.
+          - intros. cbn in *.
+            destruct l; try Result.assertion_failed_helper. cbn in *.
+            specialize (IHi (b + 1)%nat l). cbn in IHi. specialize (IHi _ H). lia.
+        Qed.
 
-    Definition range(from to: Z) := Impl.range from (Z.to_nat (to - from)).
+        Lemma completeness {F: Type} {f: Result.AssertionError F}: forall s l z, (s <= z)%nat -> (z < s + l)%nat -> exists i, Indexing.Nat.indexing (range s l) i = Success z.
+        Proof.
+          intros. remember (z - s)%nat as i.
+          exists i.
+          assert (0 <= i < l)%nat as Bounds by lia.
+          rewrite <- length with (b := s) (l := l) in Bounds.
+          destruct (Indexing.Nat.indexing (range s l) i) eqn:Eq.
+          - apply indexing in Eq. f_equal. lia.
+          - apply Indexing.Nat.failure_bounds in Eq. lia.
+        Qed.
+      End Length.
 
-    Lemma length: forall s e, length (range s e) = Z.to_nat (e - s).
-    Proof. unfold range. intros. apply Impl.length. Qed.
+      Module Bounds.
+        Definition range(from to: nat) := Length.range from (to - from)%nat.
 
-    Lemma indexing {F: Type} {f: Result.AssertionError F}: forall s e i v,
-      Indexing.Int.indexing (range s e) i = Success v -> v = (s + i).
-    Proof. unfold range. intros. apply Impl.indexing with (1 := H). Qed.
+        Lemma length: forall s e, length (range s e) = (e - s)%nat.
+        Proof. unfold range. intros. apply Length.length. Qed.
 
-    Lemma completeness {F: Type} {f: Result.AssertionError F}: forall s e z, s <= z -> z < e -> exists i, Indexing.Int.indexing (range s e) i = Success z.
-    Proof.
-      intros. remember (z - s) as i.
-      exists i.
-      assert (0 <= i < Z.of_nat (Z.to_nat (e - s))) as Bounds_z by lia.
-      rewrite <- length in Bounds_z.
-      destruct (Indexing.Int.indexing (range s e) i) eqn:Eq.
-      - apply indexing in Eq. f_equal. lia.
-      - apply Indexing.Int.failure_bounds in Eq. lia.
-    Qed.
+        Lemma indexing {F: Type} {f: Result.AssertionError F}: forall s e i v,
+          Indexing.Nat.indexing (range s e) i = Success v -> v = (s + i)%nat.
+        Proof. unfold range. intros. apply Length.indexing with (1 := H). Qed.
 
-    Lemma range_sortedness {F: Type} {f: Result.AssertionError F}: forall s e i0 i1 z0 z1,
-      (i0 <= i1)%Z ->
-      Indexing.Int.indexing (range s e) i0 = Success z0 ->
-      Indexing.Int.indexing (range s e) i1 = Success z1 ->
-      (z0 <= z1)%Z.
-    Proof. intros. apply indexing in H0. apply indexing in H1. lia. Qed.
+        Lemma completeness {F: Type} {f: Result.AssertionError F}: forall s e z, (s <= z)%nat -> (z < e)%nat -> exists i, Indexing.Nat.indexing (range s e) i = Success z.
+        Proof. unfold range. intros. apply Length.completeness; lia. Qed.
+      End Bounds.
+    End Nat.
+
+    Module Int.
+      Definition IsRange (from to: Z) (ls: list Z) :=
+        (forall (F: Type) (f: Result.AssertionError F) z, (from <= z < to)%Z -> Indexing.Int.indexing ls (z - from)%Z = Success z).
+
+      Module Length.
+        Fixpoint range (base: Z) (l: nat) := match l with
+        | 0%nat => nil
+        | S l' => base :: (range (base + 1) l')
+        end.
+
+        Lemma length: forall l b, length (range b l) = l.
+        Proof. induction l; intros b; cbn. - reflexivity. - rewrite -> IHl. reflexivity. Qed.
+
+        Lemma indexing {F: Type} {f: Result.AssertionError F}: forall i b l v,
+          Indexing.Int.indexing (range b l) i = Success v -> v = (b + i)%Z.
+        Proof.
+          induction i using pseudo_nat_ind.
+          - intros. cbn in *.
+            destruct l; try Result.assertion_failed_helper. cbn in *.
+            injection H as [=->]. lia.
+          - intros. cbn in *. rewrite -> SuccNat2Pos.id_succ in H.
+            destruct l; try Result.assertion_failed_helper. cbn in *.
+            specialize (IHi (b + 1)%Z l). cbn in IHi.
+            rewrite -> Indexing.Int.of_nat in *. specialize (IHi _ H). lia.
+          - intros. cbn in H. Result.assertion_failed_helper.
+        Qed.
+
+        Lemma completeness {F: Type} {f: Result.AssertionError F}: forall s l z, (s <= z)%Z -> (z < s + Z.of_nat l)%Z -> exists i, Indexing.Int.indexing (range s l) i = Success z.
+        Proof.
+          intros. remember (z - s)%Z as i.
+          exists i.
+          assert (0 <= i < Z.of_nat l)%Z as Bounds by lia.
+          rewrite <- length with (b := s) (l := l) in Bounds.
+          destruct (Indexing.Int.indexing (range s l) i) eqn:Eq.
+          - apply indexing in Eq. f_equal. lia.
+          - apply Indexing.Int.failure_bounds in Eq. lia.
+        Qed.
+      End Length.
+
+      Module Bounds.
+        Definition range(from to: Z) := Length.range from ( Z.to_nat (to - from)%Z ).
+
+        Lemma length: forall s e, length (range s e) = Z.to_nat (e - s)%Z.
+        Proof. unfold range. intros. apply Length.length. Qed.
+
+        Lemma indexing {F: Type} {f: Result.AssertionError F}: forall s e i v,
+          Indexing.Int.indexing (range s e) i = Success v -> v = (s + i)%Z.
+        Proof. unfold range. intros. apply Length.indexing with (1 := H). Qed.
+
+        Lemma completeness {F: Type} {f: Result.AssertionError F}: forall s e z, (s <= z)%Z -> (z < e)%Z -> exists i, Indexing.Int.indexing (range s e) i = Success z.
+        Proof. unfold range. intros. apply Length.completeness; lia. Qed.
+      End Bounds.
+    End Int.
   End Range.
 End List.
