MECMAR/props/Incorrectness.v
@@ -5,7 +5,12 @@ Import Result.Notations.
 Import Semantics.
 
 Parameter a: Character.
+Parameter b: Character.
 Axiom char_eq_refl: forall a, (a =? a = true)%Chr.
+Axiom a_b_ineq: forall a, (a =? b = false)%Chr.
+Axiom b_a_ineq: forall a, (b =? a = false)%Chr.
+
+Ltac exec := repeat( cbn || rewrite -> char_eq_refl || rewrite -> a_b_ineq || rewrite -> b_a_ineq || unfold Pos.to_nat ).
 
 Module RegexNotations.
 
@@ -16,15 +21,16 @@ Module RegexNotations.
   Notation "'</' r '/>'"  := r (r custom regex at level 99).
   Notation "r1 '|' r2" := (Disjunction r1 r2) (in custom regex at level 99, right associativity).
   Notation "r1 '~' r2" := (Seq r1 r2) (in custom regex at level 50, right associativity).
-  Notation "'(|' n ':' r '|)'" := (Group n r) (n constr at level 0, r at level 99, in custom regex at level 1).
-  Notation "'(' r ')'" := r (r at level 99, in custom regex at level 1).
+  Notation "'(' r ')'" := (Group None r) (r at level 99, in custom regex at level 1).
+  Notation "'(|' n ':' r '|)'" := (Group (Some n) r) (n constr at level 0, r at level 99, in custom regex at level 1).
+  Notation "'(?:' r ')'" := r (r at level 99, in custom regex at level 1).
   Notation "x" := x (in custom regex at level 0, x constr).
 
   Coercion Char: Character >-> Regex.
 
   Example example_1: </ a | a ~ a | a /> = Disjunction a (Disjunction (Seq a a) a). reflexivity. Qed.
-  Example example_2: </ (a | a) ~ a | a /> = Disjunction (Seq (Disjunction a a) a) a. reflexivity. Qed.
-  Example example_3: </ (|3: a |) /> = Group 3 a. reflexivity. Qed.
+  Example example_2: </ (?: a | a) ~ a | a /> = Disjunction (Seq (Disjunction a a) a) a. reflexivity. Qed.
+  Example example_3: </ ( a ) /> = Group None a. reflexivity. Qed.
 
 End RegexNotations.
 
@@ -34,10 +40,10 @@ Module Incorrectness.
   Example disjunction_commutativity: exists (r_1 r_2: Regex) (flags: RegExp) (str: list Character) (start: non_neg_integer),
     compilePattern </ r_1 | r_2 /> flags str start <> compilePattern </ r_2 | r_1 /> flags str start.
   Proof.
-    exists </ (|0: a |) />. exists </ (|1: a |) />.
-    exists (reg_exp 2).
-    exists (a :: nil). exists 0.
-    repeat( cbn || rewrite -> char_eq_refl || unfold Pos.to_nat ).
+    exists </ a ~ b />. exists </ a />.
+    exists (reg_exp 0).
+    exists (a :: b :: nil). exists 0.
+    exec.
     easy.
   Qed.
 End Incorrectness.
